Hacl HMAC: work in progress on refactoring

crypto_hst/hmac/HMAC.Masked.WIP.fst
@@ -1,4 +1,4 @@
-module HMAC
+module HMAC.Masked
   
 open FStar.Mul
 open FStar.Ghost
@@ -32,12 +32,14 @@ let uint32s = Hacl.SBuffer.u32s
 let bytes = Hacl.SBuffer.u8s
 
 
+
 (* Define operators *)
+let op_At_Plus = U32.add
 let op_At_Plus_Percent = U32.add_mod
 let op_At_Slash = U32.div
 
 (* Define parameters *)
-module HF = Hash.Sha256
+module HF = Hash.Sha256.Masked
 let hash = HF.sha256
 
 (* Get parameters *)
@@ -51,42 +53,43 @@ let hl = hashsize
 let bl = blocksize
 
 
-(* Define size of objects in the state *)
-let size_state_hash_1 = HF.size_state // UInt32s
-let size_state_hash_2 = HF.size_state // UInt32s
-
+(* Define size of objects in the state_hmac *)
 let size_key = bl // Bytes
 let size_ipad = bl // Bytes
 let size_opad = bl // Bytes
 let size_final_hash_1 = hl // Bytes
-let size_state_hmac_flat = size_key @+% size_ipad @+% size_opad @+% size_final_hash_1 // Bytes
-let size_state_hmac = size_state_hmac_flat @/ 4ul // Bytes -> UInt32s
+let size_state_hmac_flat = size_key @+ size_ipad @+ size_opad @+ size_final_hash_1 // Bytes
 
-let size_state = size_state_hash_1 @+% size_state_hash_2 @+% size_state_hmac // UInt32s
+(* Define size of objects in the state *)
+let size_state_hash_1 = HF.size_state // UInt32s
+let size_state_hash_2 = HF.size_state // UInt32s
+let size_state_hmac = size_state_hmac_flat // Bytes -> UInt32s
+let size_state = size_state_hash_1 @+ size_state_hash_2 @+ size_state_hmac // UInt32s
 
 (* Define position of objects in the state *)
 let pos_state_hash_1 = 0ul
-let pos_state_hash_2 = pos_state_hash_1 @+% size_state_hash_1
+let pos_state_hash_2 = pos_state_hash_1 @+ size_state_hash_1
+let pos_state_hmac  = pos_state_hash_2 @+ size_state_hash_2
 
-let pos_state_hmac  = pos_state_hash_2 @+% size_state_hash_2
-let pos_key         = pos_state_hmac
-let pos_ipad        = pos_key @+% size_key
-let pos_opad        = pos_ipad @+% size_ipad
-let pos_final_hash_1 = pos_opad @+% size_opad
+(* Define position of objects in state_hmac *)
+let pos_key         = 0ul
+let pos_ipad        = pos_key @+ size_key
+let pos_opad        = pos_ipad @+ size_ipad
+let pos_final_hash_1 = pos_opad @+ size_opad
 
-#set-options "--lax"
+
 
 (* Define a function to wrap the key length after bl bits *)
-val wrap_key : (okey   :bytes{length okey = U32.v bl}) -> 
-               (key    :bytes{length key % (U32.v bl) = 0 /\ disjoint okey key}) -> 
-               (keylen :u32  {U32.v keylen <= length key})
+val wrap_key : (okey   :bytes{length okey = U32.v bl}) ->
+               (key    :bytes{length key % (U32.v bl) = 0 /\ disjoint okey key}) ->
+               (keylen :s32  {S32.v keylen <= length key})
   -> STL unit
         (requires (fun h -> live h okey /\ live h key))
         (ensures  (fun h0 _ h1 -> live h1 okey /\ live h1 key /\ modifies_1 okey h0 h1))
 
 let wrap_key okey key keylen =
   if gt keylen bl then
-    hash okey key keylen
+    hash okey key keylen (uint32_to_sint32 1ul) 1ul
   else
     blit key 0ul okey 0ul keylen
 
@@ -103,29 +106,43 @@ val init' :(memb   :bytes) ->
 let init' memb state key keylen =
   (* Select the part of the state used by the inner hash function *)
   let state_hash_1 = sub state pos_state_hash_1 size_state_hash_1 in
+  let state_hash_2 = sub state pos_state_hash_2 size_state_hash_2 in
 
-  (* Initialize the underlying inner hash function *)
+  (* Initialize the underlying hash functions *)
   hash_init state_hash_1;
-  
+  hash_init state_hash_2;
+
   (* Select the part of the state used for HMAC *)
   let state_hmac = sub state pos_state_hmac size_state_hmac in
   let state_hmac_flat = sub memb 0ul size_state_hmac_flat in
+
+  (** Conversion of the hmac state back to be flatten as bytes *)
   (**) be_bytes_of_uint32s state_hmac_flat state_hmac size_state_hmac_flat;
   
-  let okey = sub state_hmac_flat pos_key size_key in
-
   (* Set initial values for ipad *)
   let ipad = sub state_hmac_flat pos_ipad size_ipad in
   setall ipad size_ipad (uint8_to_sint8 0x36uy);
+
+  (* Set initial values for ipad *)
+  let opad = sub state_hmac_flat pos_opad size_opad in
+  setall opad size_opad (uint8_to_sint8 0x5cuy);
+
+  (* Set initial values for  *)
+  let okey = sub state_hmac_flat pos_key size_key in
 
   (* Step 1: make sure the key has the proper length *)
   wrap_key okey key keylen;
 
   (* Step 2: xor "result of step 1" with ipad *)
   xor_bytes ipad okey bl;
+  xor_bytes opad okey bl;
 
   (* Step 3': feed ipad ^ okey to the inner hash function *)
-  hash_update state_hash_1 ipad size_ipad
+  hash_update state_hash_1 ipad bl (uint32_to_sint32 1ul) 1ul;
+  hash_update state_hash_2 opad bl (uint32_to_sint32 1ul) 1ul;
+
+  (** Conversion of the flat hmac state back in the global state *)
+  (**) be_uint32s_of_bytes state_hmac state_hmac_flat size_state_hmac
 
 
 val init : (state  :uint32s{length state = U32.v size_state}) ->
@@ -150,19 +167,21 @@ let init state key keylen =
   
 
 (* Update running hmac function *)
-val update : (state :uint32s) ->
-             (data  :bytes {disjoint state data}) ->
-             (len   :u32)
+val update : (state :uint32s{length state = U32.v size_state}) ->
+             (data    :bytes{ length data >= U32.v blocksize /\ (length data) % (U32.v blocksize) = 0 /\ disjoint data state}) ->
+             (len     :s32{S32.v len + 8 < pow2 32 /\ S32.v len <= length data}) ->
+             (rounds_data:s32{S32.v rounds_data * U32.v blocksize < pow2 32}) ->
+             (rounds_mask:u32{U32.v rounds_mask * U32.v blocksize = length data})
              -> STL unit
                   (requires (fun h -> live h state /\ live h data))
                   (ensures  (fun h0 r h1 -> live h1 state /\ live h1 data /\ modifies_1 state h0 h1))
 
-let update state data len =
+let update state data len rounds_data rounds_mask =
   (* Select the part of the state used by the inner hash function *)
   let state_hash_1 = sub state pos_state_hash_1 size_state_hash_1 in
   
   (* Step 3'' and Step 4: Feed the message to the inner hash function *)
-  hash_update state_hash_1 data len
+  hash_update state_hash_1 data len rounds_data rounds_mask
 
 
 
@@ -177,33 +196,23 @@ val finish': (memb  :bytes) ->
 let finish' memb mac state =
   (* Select the part of the state used by the inner hash function *)
   let state_hash_1 = sub state pos_state_hash_1 size_state_hash_1 in
-
-  (* Select the part of the state used by the outter hash function *)
   let state_hash_2 = sub state pos_state_hash_2 size_state_hash_2 in
 
-  (* Initialize the underlying outer hash function *)
-  hash_init state_hash_2;
-  
   (* Select the part of the state used for HMAC *)
   let state_hmac = sub state pos_state_hmac size_state_hmac in
   let state_hmac_flat = sub memb 0ul size_state_hmac_flat in
-
+  
+  (* Select the part of the state used for the inner final hash *)
   let final_hash_1 = sub state_hmac_flat pos_final_hash_1 size_final_hash_1 in
-  let okey = sub state_hmac_flat pos_key size_key in
 
-  (* Set initial values for opad *)
-  let opad = sub state_hmac_flat pos_opad size_opad in
-  setall opad size_opad (uint8_to_sint8 0x5cuy);
-
-  (* Step 5: xor "result of step 1" with opad *)
-  xor_bytes opad okey size_opad;
+  (** Conversion of the hmac state back to be flatten as bytes *)
+  (**) be_bytes_of_uint32s state_hmac_flat state_hmac size_state_hmac_flat;
 
   (* Step 6: finalize inner hash *)
   hash_finish final_hash_1 state_hash_1;
 
   (* Step 6': feed (opad ^ okey) and the final inner hash to the outer hash *)
-  hash_update state_hash_2 opad size_opad;
-  hash_update state_hash_2 final_hash_1 hashsize;
+  hash_update state_hash_2 final_hash_1 hashsize (uint32_to_sint32 1ul) 1ul;
 
   (* Step 7: finalize outer hash to compute the final mac *)
   hash_finish mac state_hash_2
@@ -235,16 +244,19 @@ val hmac_core': (memb   :uint32s) ->
                 (mac    :bytes { length mac >= U32.v hashsize /\ disjoint mac memb}) ->
                 (key    :bytes { disjoint key memb /\ disjoint key mac }) ->
                 (keylen :u32   { length key = U32.v keylen }) ->
-                (data   :bytes { disjoint data memb /\ disjoint data mac /\ disjoint data key }) ->
-                (len    :u32   { length data = U32.v len })
+                (data    :bytes{ length data >= U32.v blocksize /\ (length data) % (U32.v blocksize) = 0
+                                   /\ disjoint data memb /\ disjoint data hash}) ->
+                (len     :s32{S32.v len + 8 < pow2 32 /\ S32.v len <= length data}) ->
+                (rounds_data:s32{S32.v rounds_data * U32.v blocksize < pow2 32}) ->
+                (rounds_mask:u32{U32.v rounds_mask * U32.v blocksize = length data})
                 -> STL unit
                       (requires (fun h -> live h mac /\ live h key /\ live h data))
                       (ensures  (fun h0 r h1 -> live h1 memb /\ live h1 mac /\ modifies_2 memb mac h0 h1))
 
-let hmac_core' memb mac key keylen data len =
+let hmac_core' memb mac key keylen data len rounds_data rounds_len =
   let state = memb in
   init state key keylen;
-  update state data len;
+  update state data len rounds_data rounds_len;
   finish mac state
 
 
@@ -252,26 +264,26 @@ let hmac_core' memb mac key keylen data len =
 val hmac_core: (mac    :bytes {length mac >= U32.v hashsize }) ->
                (key    :bytes {length key % (U32.v bl) = 0 /\ disjoint key mac }) ->
                (keylen :u32   {U32.v keylen <= length key}) ->
-               (data   :bytes {length key % (U32.v bl) = 0 /\ disjoint data mac /\ disjoint data key }) ->
-               (len    :u32   {U32.v len <= length data})
+               (data    :bytes{ length data >= U32.v blocksize /\ (length data) % (U32.v blocksize) = 0
+                                   /\ disjoint data memb /\ disjoint data hash}) ->
+               (len     :s32{S32.v len + 8 < pow2 32 /\ S32.v len <= length data}) ->
+               (rounds_data:s32{S32.v rounds_data * U32.v blocksize < pow2 32}) ->
+               (rounds_mask:u32{U32.v rounds_mask * U32.v blocksize = length data})
                -> STL unit
                      (requires (fun h -> live h mac /\ live h key /\ live h data))
                      (ensures  (fun h0 r h1 -> live h1 mac /\ modifies_1 mac h0 h1))
 
-let hmac_core mac key keylen data len =
+let hmac_core mac key keylen data len rounds_data rounds_mask =
 
   (** Push frame *)
   (**) push_frame();
 
-  (* Compute size of objects *)
-  let _statelen = size_state in
-
   (* Allocate the memory block for the underlying function *)
-  let memblen = _statelen in
+  let memblen = size_state in
   let memb = create (uint32_to_sint32 0ul) memblen in
 
   (* Call the hmac function *)
-  hmac_core' memb mac key keylen data len ;
+  hmac_core' memb mac key keylen data len rounds_data rounds_mask;
 
   (** Pop frame *)
   (**) pop_frame()
@@ -282,11 +294,14 @@ let hmac_core mac key keylen data len =
 val hmac_sha256 : (mac     :bytes { length mac = U32.v hl }) ->
                   (key     :bytes { disjoint key mac }) ->
                   (keylen  :u32   { length key = U32.v keylen }) ->
-                  (data    :bytes { disjoint mac data }) ->
-                  (datalen :u32   {5 * U32.v bl + U32.v hl + U32.v datalen < pow2 32 /\ length data = U32.v datalen /\ U32.v datalen + U32.v bl <= pow2 32})
+                  (data    :bytes{ length data >= U32.v blocksize /\ (length data) % (U32.v blocksize) = 0
+                                   /\ disjoint data memb /\ disjoint data hash}) ->
+                  (len     :s32{S32.v len + 8 < pow2 32 /\ S32.v len <= length data}) ->
+                  (rounds_data:s32{S32.v rounds_data * U32.v blocksize < pow2 32}) ->
+                  (rounds_mask:u32{U32.v rounds_mask * U32.v blocksize = length data})
                   -> STL unit
                         (requires (fun h -> live h mac /\ live h data /\ live h key))
                         (ensures  (fun h0 r h1 -> live h1 mac /\ modifies_1 mac h0 h1))
 
-let hmac_sha256 mac key keylen data datalen = hmac_core mac key keylen data datalen
+let hmac_sha256 mac key keylen data len rounds_data rounds_mask = hmac_core mac key keylen data len rounds_data rounds_mask
 
